src/IndexedToCoind.v
@@ -3,7 +3,6 @@ Import List.ListNotations.
 Open Scope list_scope.
 From Coq Require Import Setoid.
 From Coq Require Import Morphisms.
-From Coq Require Import NPeano.
 From Coq Require Import Program.Tactics.
 
 From Velus Require Import Common.
