src/Obc/Equiv.v
@@ -272,7 +272,7 @@ Module Type EQUIV
     intros Pc P p1 p2 WTp Types Externs Hfa Hclasses.
     rewrite program_refines_def; split; [|split]; auto.
     unfold find_class.
-    pose proof (Forall2_length _ _ _ Hfa) as Hlen.
+    pose proof (@Forall2_length _ _ _ _ _ Hfa) as Hlen.
     revert WTp Hfa Hclasses.
     destruct p1, p2; simpl in *; subst.
     pattern classes0, classes1.
